src/Monoid.v
@@ -2,7 +2,8 @@
 
 Unset Automatic Introduction.
 Require Import Foundations.hlevel2.algebra1b
-        Ktheory.Utilities.
+	       RezkCompletion.auxiliary_lemmas_HoTT
+               Ktheory.Utilities.
 Require Ktheory.Magma Ktheory.QuotientSet.
 Import RezkCompletion.pathnotations.PathNotations Ktheory.Utilities.Notation. 
 Local Notation Hom := monoidfun (only parsing).
@@ -47,8 +48,18 @@ Module Presentation.
   (** ** premonoids over X
          A pre-monoid over X modulo an adequate relation over R will be a
          monoid M equipped with a map X -> M that respects the relations R. *)
-  Require Import RezkCompletion.auxiliary_lemmas_HoTT.
-  Record MarkedPremonoid X := 
+  Inductive word X : Type :=
+    | word_unit : word X
+    | word_gen : X -> word X 
+    | word_op : word X -> word X -> word X.
+  Arguments word_unit {X}.
+  Arguments word_gen {X} x.
+  Arguments word_op {X} v w.
+  Record reln X := make_reln { lhs : word X; rhs : word X }.
+  Arguments lhs {X} r.
+  Arguments rhs {X} r.
+  Arguments make_reln {X} _ _.
+  Record MarkedPreMonoid X := 
     make_preMonoid {
         elem :> Type;
         op0 : elem;
@@ -59,19 +70,17 @@ Module Presentation.
   Arguments op1 {X M} x : rename.
   Arguments op2 {X M} v w : rename.
   Definition wordop X := make_preMonoid X (word X) word_unit word_gen word_op.
-  Definition evalword' {X} (Y:MarkedPremonoid X) (w:word X) : elem Y.
-    intros ? Y w. induction w as [|x|_ x _ y].
-    { exact op0. } { exact (op1 x). } { exact (op2 x y). } Defined.
-  Fixpoint evalword {X} (Y:MarkedPremonoid X) (w:word X) : elem Y.
+  Fixpoint evalword {X} (Y:MarkedPreMonoid X) (w:word X) : elem Y.
     intros ? Y [|x|v w]. { exact op0. } { exact (op1 x). }
     { exact (op2 (evalword X Y v) (evalword X Y w)). } Defined.
-  Definition MarkedPremonoid_to_hrel {X} (M:MarkedPremonoid X) (is:isaset (elem M)) : 
+  Definition MarkedPreMonoid_to_hrel {X} 
+             (M:MarkedPreMonoid X) (is:isaset (elem M)) : 
       hrel (word X) :=
     fun v w => (evalword M v == evalword M w) ,, is _ _.
   (** eta expansion principle for words *)
-  Lemma reassemble {X I} (R:I->reln X) (v:wordop X) : evalword (wordop X) v == v.
-  Proof. intros. induction v as [|x|v v' w w']. 
-         { reflexivity. } { reflexivity. } { exact (aptwice word_op v' w'). } Qed.
+  Fixpoint reassemble {X I} (R:I->reln X) (v:wordop X) : evalword (wordop X) v == v.
+  Proof. intros ? ? ? [|x|v w]. { reflexivity. } { reflexivity. }
+         { exact (aptwice word_op (reassemble _ _ R v) (reassemble _ _ R w)). } Qed.
   (** ** adequate relations over R *)
   Record AdequateRelation {X I} (R:I->reln X) (r : hrel (word X)) := 
     make_AdequateRelation {
@@ -83,7 +92,8 @@ Module Presentation.
         right_compat: forall u v w, r u v -> r (word_op u w) (word_op v w);
         left_unit : forall w, r (word_op word_unit w) w;
         right_unit : forall w, r (word_op w word_unit) w;
-        assoc : forall u v w, r (word_op (word_op u v) w) (word_op u (word_op v w)) }.
+        assoc : forall u v w, r (word_op (word_op u v) w) (word_op u (word_op v w))
+      }.
   Arguments make_AdequateRelation {X I} R r _ _ _ _ _ _ _ _ _.
   Arguments base {X I R r} _ _.
   Definition adequacy_to_eqrel {X I} (R:I->reln X) (r : hrel (word X)) :
@@ -94,7 +104,7 @@ Module Presentation.
   (** ** the smallest adequate relation over R 
          It is defined as the intersection of all the adequate relations.
          Later we'll have to deal with the "resizing" to resolve issues
-         with universes. *)
+         withe universes. *)
   Definition smallestAdequateRelation0 {X I} (R:I->reln X) : hrel (word X).
     intros ? ? ? v w.
     exists (forall r: hrel (word X), AdequateRelation R r -> r v w).
@@ -111,11 +121,12 @@ Module Presentation.
          { intros ? ? ? p r ra. apply (right_compat R). exact ra. exact (p r ra). }
          { intros ? r ra. apply (left_unit R). exact ra. }
          { intros ? r ra. apply (right_unit R). exact ra. }
-         { exact (fun u v w r ra => assoc R r ra u v w). } Qed.
+         { exact (fun u v w r ra => assoc R r ra u v w). } 
+  Qed.
   Definition smallestAdequateRelation {X I} (R:I->reln X) : eqrel (word X).
     intros. exact (adequacy_to_eqrel R _ (adequacy R)). Defined.
-  (** *** the underlying set of the monoid with generators X and relations R *)
-  Definition universalMarkedPremonoid0 {X I} (R:I->reln X) : hSet := 
+  (** *** the underlying set of the abelian group with generators X and relations R *)
+  Definition universalMarkedPreMonoid0 {X I} (R:I->reln X) : hSet := 
     setquotinset (smallestAdequateRelation R).
   Lemma op2_compatibility {X I} (R:I->reln X) : 
     QuotientSet.iscomprelrelfun2
@@ -125,69 +136,71 @@ Module Presentation.
     { intros x x' y p r ra. exact (right_compat R r ra x x' y (p r ra)). }
     { intros x y y' p r ra. exact ( left_compat R r ra x y y' (p r ra)). } Qed.
   (** *** the multiplication on on it *)
-  Definition univ_binop {X I} (R:I->reln X) : binop (universalMarkedPremonoid0 R).
+  Definition univ_binop {X I} (R:I->reln X) : binop (universalMarkedPreMonoid0 R).
     intros. refine (QuotientSet.setquotfun2 word_op _). apply op2_compatibility. Defined.
   Definition univ_setwithbinop {X I} (R:I->reln X) : setwithbinop
-             := setwithbinoppair (universalMarkedPremonoid0 R) (univ_binop R).
-  (** *** the universal premonoid *)
-  Definition universalMarkedPremonoid {X I} (R:I->reln X) : MarkedPremonoid X.
-    intros. refine (make_preMonoid X (universalMarkedPremonoid0 R) _ _ _).
+             := setwithbinoppair (universalMarkedPreMonoid0 R) (univ_binop R).
+  (** *** the universal pre- group *)
+  Definition universalMarkedPreMonoid {X I} (R:I->reln X) : MarkedPreMonoid X.
+    intros. refine (make_preMonoid X (universalMarkedPreMonoid0 R) _ _ _).
     { exact (setquotpr _ word_unit). }
     { exact (fun x => setquotpr _ (word_gen x)). }
     { exact (univ_binop _). } Defined.
-  (** *** identities for the universal premonoid *)
-  Lemma is_left_unit_univ_binop {X I} (R:I->reln X) : 
-    forall w : universalMarkedPremonoid0 R, ((univ_binop _) (setquotpr _ word_unit) w) == w.
-  Proof. intros ? ? ? w'. assert (lift := issurjsetquotpr (smallestAdequateRelation R)).
-    apply (squash_to_prop (lift w')).
-    { apply setproperty. } 
-    { intros [w []].
-      exact (iscompsetquotpr (smallestAdequateRelation R) _ _ 
-                             (fun r ra => left_unit R r ra w)). } Qed.
-  Lemma is_right_unit_univ_binop {X I} (R:I->reln X) : 
-    forall w : universalMarkedPremonoid0 R, ((univ_binop _) w (setquotpr _ word_unit)) == w.
-  Proof. intros ? ? ? w'. assert (lift := issurjsetquotpr (smallestAdequateRelation R)).
-    isaprop_goal ig. { apply setproperty. } 
-    apply (squash_to_prop (lift w') ig); intros [w []].
+  (** *** identities for the universal preabelian group *)
+  Lemma lift {X I} (R:I->reln X) : issurjective (setquotpr (smallestAdequateRelation R)).
+  Proof. intros. exact (issurjsetquotpr (smallestAdequateRelation R)). Qed.
+  Lemma is_left_unit_univ_binop {X I} (R:I->reln X) (w:universalMarkedPreMonoid0 R) :
+    ((univ_binop _) (setquotpr _ word_unit) w) == w.
+  Proof. intros ? ? ? w'. isaprop_goal ig. { apply setproperty. } 
+    apply (squash_to_prop (lift R w') ig); intros [w []].
+    exact (iscompsetquotpr (smallestAdequateRelation R) _ _ 
+                           (fun r ra => left_unit R r ra w)). Qed.
+  Lemma is_right_unit_univ_binop {X I} (R:I->reln X) (w:universalMarkedPreMonoid0 R) :
+    ((univ_binop _) w (setquotpr _ word_unit)) == w.
+  Proof. intros ? ? ? w'. isaprop_goal ig. { apply setproperty. } 
+    apply (squash_to_prop (lift R w') ig); intros [w []].
     exact (iscompsetquotpr (smallestAdequateRelation R) _ _ 
                            (fun r ra => right_unit R r ra w)). Qed.
   Lemma isassoc_univ_binop {X I} (R:I->reln X) : isassoc(univ_binop R).
   Proof. intros. set (e := smallestAdequateRelation R). intros u' v' w'. 
-         isaprop_goal ig. { apply setproperty. } assert (lift := issurjsetquotpr e).
-         apply (squash_to_prop (lift u') ig); intros [u i]; destruct i.
-         apply (squash_to_prop (lift v') ig); intros [v j]; destruct j.
-         apply (squash_to_prop (lift w') ig); intros [w []].
+         isaprop_goal ig. { apply setproperty. } 
+         apply (squash_to_prop (lift R u') ig); intros [u i]; destruct i.
+         apply (squash_to_prop (lift R v') ig); intros [v j]; destruct j.
+         apply (squash_to_prop (lift R w') ig); intros [w []].
          exact (iscompsetquotpr e _ _ (fun r ra => assoc R r ra u v w)). Qed.
-  Lemma reassemble_pr {X I} (R:I->reln X) (v:word X) : 
-    evalword (universalMarkedPremonoid R) v == setquotpr _ v.
-  Proof. intros. induction v as [|x|v v' w w']. { reflexivity. } { reflexivity. }
-         { simpl. assert (p := ! v'); destruct p; clear v'.
-                  assert (q := ! w'); destruct q; clear w'. reflexivity. } Qed.
+  Fixpoint reassemble_pr {X I} (R:I->reln X) (v:word X) : 
+    evalword (universalMarkedPreMonoid R) v == setquotpr _ v.
+  Proof. intros ? ? ? [|x|v w]. { reflexivity. } { reflexivity. }
+         { simpl. assert (p := ! reassemble_pr _ _ R v). destruct p.
+                  assert (q := ! reassemble_pr _ _ R w). destruct q.
+                  reflexivity. } Qed.
   Lemma pr_eval_compat {X I} (R:I->reln X) (w:word X) :
     setquotpr (smallestAdequateRelation R) (evalword (wordop X) w) 
-    == evalword (universalMarkedPremonoid R) w.
+    == evalword (universalMarkedPreMonoid R) w.
   Proof. intros. destruct w as [|x|v w]. { reflexivity. } { reflexivity. } 
     { assert (p := !reassemble R (word_op v w)). destruct p. 
       exact (!reassemble_pr R (word_op v w)). } Qed.
-  (** *** monoids over X modulo R *)
-  Definition toMarkedPremonoid {X I} (R:I->reln X) (M:monoid) (el:X->M) : MarkedPremonoid X.
-    intros. exact {| elem := M; op0 := unel _; op1 := el; op2 := op |}. Defined.
+  (** *** abelian groups over X modulo R *)
+  Definition toMarkedPreMonoid {X I} (R:I->reln X) (M:monoid) (el:X->M) : 
+      MarkedPreMonoid X.
+    intros. exact {| elem := M; op0 := unel _; op1 := el; op2 := op |}.
+  Defined.
   Record MarkedMonoid {X I} (R:I->reln X) := 
     make_MarkedMonoid {
         m_base :> monoid;
         m_mark : X -> m_base;
-        m_reln : forall i, evalword (toMarkedPremonoid R m_base m_mark) (lhs (R i)) ==
-                           evalword (toMarkedPremonoid R m_base m_mark) (rhs (R i)) }.
+        m_reln : forall i, evalword (toMarkedPreMonoid R m_base m_mark) (lhs (R i)) ==
+                           evalword (toMarkedPreMonoid R m_base m_mark) (rhs (R i)) }.
   Arguments make_MarkedMonoid {X I} R _ _ _.
   Arguments m_base {X I R} _.
   Arguments m_mark {X I R} _ x.
-  Definition toMarkedPremonoid' {X I} {R:I->reln X} (M:MarkedMonoid R) : MarkedPremonoid X :=
-    toMarkedPremonoid R (m_base M) (m_mark M).
+  Definition toMarkedPreMonoid' {X I} {R:I->reln X} (M:MarkedMonoid R) : MarkedPreMonoid X :=
+    toMarkedPreMonoid R (m_base M) (m_mark M).
   Definition evalwordMM {X I} {R:I->reln X} (M:MarkedMonoid R) : word X -> M :=
-    evalword (toMarkedPremonoid' M).
+    evalword (toMarkedPreMonoid' M).
   Definition MarkedMonoid_to_hrel {X I} {R:I->reln X} (M:MarkedMonoid R) : hrel (word X) :=
     fun v w  => eqset (evalwordMM M v) (evalwordMM M w).
-  Lemma monoid_adequacy {X I} (R:I->reln X) (M:MarkedMonoid R) :
+  Lemma abelian_group_adequacy {X I} (R:I->reln X) (M:MarkedMonoid R) :
     AdequateRelation R (MarkedMonoid_to_hrel M).
   Proof. intros. refine (make_AdequateRelation R _ _ _ _ _ _ _ _ _ _).
          { exact (fun i => m_reln R M i). } { reflexivity. }
@@ -196,7 +209,8 @@ Module Presentation.
            unfold evalwordMM,evalword in *. destruct p. reflexivity. }
          { intros ? ? ? p. simpl in p; simpl. 
            unfold evalwordMM,evalword in *. destruct p. reflexivity. }
-         { intros. apply lunax. } { intros. apply runax. } { intros. apply assocax. } Qed.
+         { intros. apply lunax. } { intros. apply runax. } { intros. apply assocax. } 
+  Qed.
   Record MarkedMonoidMap {X I} {R:I->reln X} (M N:MarkedMonoid R) :=
     make_MarkedMonoidMap {
         map_base :> Hom M N;
@@ -209,28 +223,33 @@ Module Presentation.
          destruct f as [f ft], g as [g gt]; simpl in j. destruct j.
          assert(k : ft == gt). { apply funextsec; intro x. apply setproperty. } destruct k. 
          reflexivity. Qed.
-  Lemma MarkedMonoidMap_compat {X I} {R:I->reln X}
+  Fixpoint MarkedMonoidMap_compat {X I} {R:I->reln X}
            {M N:MarkedMonoid R} (f:MarkedMonoidMap M N) (w:word X) :
     map_base f (evalwordMM M w) == evalwordMM N w.
-  Proof. intros. induction w as [|x|v v' w w'].
+  Proof. intros. destruct w as [|x|v w].
          { exact (unitproperty f). }
          { exact (map_mark f x). }
          { exact (multproperty f (evalwordMM M v) (evalwordMM M w)
-                  @ aptwice (fun r s => r * s) v' w'). } Qed.
+                  @ aptwice (fun r s => r * s) 
+                            (MarkedMonoidMap_compat _ _ _ _ _ f v) 
+                            (MarkedMonoidMap_compat _ _ _ _ _ f w)). } Qed.
   Lemma MarkedMonoidMap_compat2 {X I} {R:I->reln X} 
            {M N:MarkedMonoid R} (f g:MarkedMonoidMap M N) (w:word X) :
     map_base f (evalwordMM M w) == map_base g (evalwordMM M w).
-  Proof. intros. exact (MarkedMonoidMap_compat f w @ !MarkedMonoidMap_compat g w). Qed.
-  (** *** the universal marked monoid over X modulo R *)
+  Proof. intros. 
+         exact (MarkedMonoidMap_compat f w @ !MarkedMonoidMap_compat g w). Qed.
+  (** *** the universal marked abelian group over X modulo R *)
   Definition universalMarkedMonoid0 {X I} (R:I->reln X) : monoid.
     intros. 
-    { exists (univ_setwithbinop R). split.
-      { exact (isassoc_univ_binop R). }
-      { exists (setquotpr _ word_unit). split. 
-        { exact (is_left_unit_univ_binop R). }
-        { exact (is_right_unit_univ_binop R). } } } Defined.
-  Definition universalMarkedMonoid1 {X I} (R:I->reln X) : MarkedPremonoid X :=
-    (toMarkedPremonoid R 
+    { exists (univ_setwithbinop R). 
+        { split.
+          { exact (isassoc_univ_binop R). }
+          { exists (setquotpr _ word_unit). split. 
+            { exact (is_left_unit_univ_binop R). }
+            { exact (is_right_unit_univ_binop R). } } } }
+Defined.
+  Definition universalMarkedMonoid1 {X I} (R:I->reln X) : MarkedPreMonoid X :=
+    (toMarkedPreMonoid R 
                   (universalMarkedMonoid0 R)
                   (fun x : X => setquotpr (smallestAdequateRelation R) (word_gen x))). 
   Lemma universalMarkedMonoid2 {X I} (R:I->reln X) (w:word X) : 
@@ -249,40 +268,73 @@ Module Presentation.
     make_MarkedMonoid R (universalMarkedMonoid0 R) 
                 (fun x => setquotpr (smallestAdequateRelation R) (word_gen x)) 
                 (universalMarkedMonoid3 R).
+  Fixpoint agreement_on_gens0 {X I} {R:I->reln X} {M:monoid}
+        (f g:Hom (universalMarkedMonoid R) M)
+        (p:forall i, f (setquotpr (smallestAdequateRelation R) (word_gen i)) ==
+                   g (setquotpr (smallestAdequateRelation R) (word_gen i)))
+        (w:word X) :
+          pr1 f (setquotpr (smallestAdequateRelation R) w) ==
+          pr1 g (setquotpr (smallestAdequateRelation R) w).
+  Proof. intros. destruct w as [|x|v w].
+         { intermediate (unel M). exact (unitproperty f). exact (!unitproperty g). }
+         { apply p. }
+         (* compare duplication with the proof of MarkedMonoidMap_compat *)
+         { refine (
+               multproperty f (setquotpr (smallestAdequateRelation R) v)
+                   (setquotpr (smallestAdequateRelation R) w)
+             @ _ @ !
+               multproperty g (setquotpr (smallestAdequateRelation R) v)
+                   (setquotpr (smallestAdequateRelation R) w)).
+           apply (aptwice (fun r s => r * s)).
+           { apply agreement_on_gens0. assumption. }
+           { apply agreement_on_gens0. assumption. } } Qed.
+  Lemma agreement_on_gens {X I} {R:I->reln X} {M:monoid}
+        (f g:Hom (universalMarkedMonoid R) M) :
+        (forall i, f (setquotpr (smallestAdequateRelation R) (word_gen i)) ==
+                   g (setquotpr (smallestAdequateRelation R) (word_gen i))) 
+          -> f == g.
+    intros ? ? ? ? ? ? p. apply funEquality.
+    apply funextfunax; intro t; simpl in t. 
+    apply (surjectionisepitosets _ _ _ (issurjsetquotpr _)).
+    { apply setproperty. } { apply agreement_on_gens0. assumption. } Qed.
   Definition universality0 {X I} {R:I->reln X} (M:MarkedMonoid R) : 
     universalMarkedMonoid0 R -> M.
   Proof. intros ? ? ? ?. 
     apply (setquotuniv _ _ (evalwordMM M)).
-    exact (fun _ _ r => r (MarkedMonoid_to_hrel M) (monoid_adequacy R M)).
+    exact (fun _ _ r => r (MarkedMonoid_to_hrel M) (abelian_group_adequacy R M)).
   Defined.
   Definition universality1 {X I} (R:I->reln X) 
                            (M:MarkedMonoid R) (v w:universalMarkedMonoid0 R) :
     universality0 M (v * w) == universality0 M v * universality0 M w.
-  Proof. intros.
-         assert (lift := issurjsetquotpr (smallestAdequateRelation R)).
-         isaprop_goal ig. { apply setproperty. }
-         apply (squash_to_prop (lift v) ig); intros [v' j]; destruct j.
-         apply (squash_to_prop (lift w) ig); intros [w' []].
-         reflexivity. Qed.
+  Proof. intros. isaprop_goal ig. { apply setproperty. }
+    apply (squash_to_prop (lift R v) ig); intros [v' j]; destruct j.
+    apply (squash_to_prop (lift R w) ig); intros [w' []].
+    reflexivity. Qed.
   Definition universality2 {X I} {R:I->reln X} (M:MarkedMonoid R) : 
     monoidfun (universalMarkedMonoid R) M.
   Proof. intros. exists (universality0 M).
       split. { intros v w. apply universality1. } { reflexivity. } Defined.
-  (** * universality of the universal marked monoid *)
+  (** * universality of the universal marked abelian group *)
   Local Arguments pr1monoidfun {X Y} f x.
   Theorem iscontrMarkedMonoidMap {X I} {R:I->reln X} (M:MarkedMonoid R) :
         iscontr (MarkedMonoidMap (universalMarkedMonoid R) M).
-  Proof. intros. assert (g := make_MarkedMonoidMap X I R (universalMarkedMonoid R) M 
-                                             (universality2 M) (fun x => idpath _)).
-         exists g. intros f. apply MarkedMonoidMapEquality.
-         apply funEquality. apply funextfunax; intro v.
-         assert (lift := issurjsetquotpr (smallestAdequateRelation R)).
-         isaprop_goal ig. { apply setproperty. }
-         apply (squash_to_prop (lift v) ig); intros [w []].
-         exact ((ap f (universalMarkedMonoid2 R w)) 
-              @ MarkedMonoidMap_compat2 f g w @ !(ap g (universalMarkedMonoid2 R w))).
-         Qed.
+  Proof. intros. 
+    assert (g := make_MarkedMonoidMap X I R 
+                           (universalMarkedMonoid R) M 
+                           (universality2 M) (fun x => idpath _)).
+    exists g. intros f. apply MarkedMonoidMapEquality.
+    apply funEquality. apply funextfunax; intro v.
+    isaprop_goal ig. { apply setproperty. }
+    apply (squash_to_prop (lift R v) ig); intros [w []].
+    exact ((ap f (universalMarkedMonoid2 R w)) 
+         @ MarkedMonoidMap_compat2 f g w @ !(ap g (universalMarkedMonoid2 R w))).
+  Defined.
 End Presentation.
+Module Free.
+  Import Presentation.
+  Definition make (X:Type) : monoid := @universalMarkedMonoid X empty fromempty.
+End Free.
+Definition NN := Free.make unit.
 Module Product.
   Definition make {I} (X:I->monoid) : monoid.
     intros. exists (Magma.Product.make X). split.
